from serializers to leaf writers

src/lowparse/LowParse.Low.Base.fst
@@ -1111,6 +1111,68 @@ let leaf_writer_strong
     valid_content_pos p h' sl pos x pos'
   ))
 
+inline_for_extraction
+let serializer32
+  (#k: parser_kind)
+  (#t: Type)
+  (#p: parser k t)
+  (s: serializer p)
+: Tot Type
+= (x: t) ->
+  (b: buffer8) ->
+  HST.Stack U32.t
+  (requires (fun h -> B.live h b /\ Seq.length (serialize s x) <= B.length b))
+  (ensures (fun h len h' ->
+    Seq.length (serialize s x) == U32.v len /\ (
+    let b' = B.gsub b 0ul len in
+    B.modifies (B.loc_buffer b') h h' /\
+    B.live h b /\
+    B.as_seq h' b' `Seq.equal` serialize s x
+  )))
+
+inline_for_extraction
+let leaf_writer_strong_of_serializer32
+  (#k: parser_kind)
+  (#t: Type)
+  (#p: parser k t)
+  (#s: serializer p)
+  (s32: serializer32 s)
+  (u: squash (k.parser_kind_subkind == Some ParserStrong))
+: Tot (leaf_writer_strong s)
+= fun x input pos ->
+  let b = B.sub input.base pos (input.len `U32.sub` pos) in
+  let len = s32 x b in
+  let h = HST.get () in
+  [@inline_let] let pos' = pos `U32.add` len in
+  [@inline_let] let _ : squash (valid_content_pos p h input pos x pos') =
+    let small = B.as_seq h (B.gsub b 0ul len) in
+    let large = B.as_seq h b in
+    assert (no_lookahead_on p small large);
+    assert (injective_postcond p small large);
+    valid_facts p h input pos;
+    ()
+  in
+  pos'
+
+inline_for_extraction
+let leaf_writer_weak_of_strong_constant_size
+  (#k: parser_kind)
+  (#t: Type)
+  (#p: parser k t)
+  (#s: serializer p)
+  (s32: leaf_writer_strong s)
+  (sz: U32.t)
+  (u: squash (
+    k.parser_kind_high == Some k.parser_kind_low /\
+    k.parser_kind_low == U32.v sz /\
+    k.parser_kind_low < U32.v max_uint32
+  ))
+: Tot (leaf_writer_weak s)
+= fun x input pos ->
+  if (input.len `U32.sub` pos) `U32.lt` sz
+  then max_uint32
+  else s32 x input pos
+
 #set-options "--z3rlimit 16"
 
 inline_for_extraction
@@ -1469,366 +1531,3 @@ let valid_exact_ext_elim
   ))
 = assert (injective_precond p (B.as_seq h (B.gsub s1.base pos1 (pos1' `U32.sub` pos1))) (B.as_seq h (B.gsub s2.base pos2 (pos2' `U32.sub` pos2))));
   assert (injective_postcond p (B.as_seq h (B.gsub s1.base pos1 (pos1' `U32.sub` pos1))) (B.as_seq h (B.gsub s2.base pos2 (pos2' `U32.sub` pos2))))
-
-(*
-module I32 = FStar.Int32
-module Cast = FStar.Int.Cast
-module MA = LowParse.Math
-
-let int32_to_uint32_pos
-  (x: I32.t)
-: Lemma
-  (requires (I32.v x >= 0))
-  (ensures (U32.v (Cast.int32_to_uint32 x) == I32.v x))
-  [SMTPat (U32.v (Cast.int32_to_uint32 x))]
-= MA.modulo_lemma (I32.v x) (pow2 32)
-
-let uint32_to_int32_bounded
-  (x: U32.t)
-: Lemma
-  (requires (U32.v x < 2147483648))
-  (ensures (I32.v (Cast.uint32_to_int32 x) == U32.v x))
-  [SMTPat (I32.v (Cast.uint32_to_int32 x))]
-= MA.modulo_lemma (U32.v x) (pow2 32)
-
-inline_for_extraction
-type pointer (t: Type) = (b: B.buffer t { B.length b == 1 } )
-
-let is_slice (h: HS.mem) (#t: Type) (b: B.buffer t) (len: I32.t) : GTot Type0 =
-  B.live h b /\
-  B.length b == I32.v len
-
-unfold
-let gsub
-  (#t: Type)
-  (b: B.buffer t)
-  (i: U32.t)
-  (len: U32.t)
-: Ghost (B.buffer t)
-  (requires (U32.v i + U32.v len <= B.length b))
-  (ensures (fun b' -> B.length b' == U32.v len))
-= B.gsub b i len
-
-let is_tail_of (#t: Type) (b' b : B.buffer t) : GTot Type0 =
-  B.length b' <= B.length b /\
-  b' == gsub b (U32.uint_to_t (B.length b - B.length b')) (U32.uint_to_t (B.length b'))
-
-let tail_ptr (h h' : HS.mem) (#t: Type) (p: pointer (B.buffer t)) : GTot Type0 =
-  B.live h p /\
-  B.live h' p /\ (
-    let b = B.get h p 0 in
-    let b' = B.get h' p 0 in
-    B.live h b /\
-    B.live h' b /\
-    b' `is_tail_of` b
-  )
-
-let parse_from_slice
-  (#k: parser_kind)
-  (#t: Type0)
-  (p: parser k t)
-  (h: HS.mem)
-  (b: buffer8)
-  (sz: I32.t)
-: Ghost (option (t * nat))
-  (requires (is_slice h b sz))
-  (ensures (fun y ->
-    match y with
-    | None -> parse p (B.as_seq h b) == None
-    | Some (x, len) -> len <= B.length b /\ parse p (B.as_seq h b) == Some (x, len)
-  ))
-= match parse p (B.as_seq h b) with
-  | Some (x, len) -> Some (x, len)
-  | _ -> None
-
-(* A validator, if succeeds, returns the remaining length; otherwise returns a negative number. *)
-
-let validator32_postcond
-  (#k: parser_kind)
-  (#t: Type0)
-  (p: parser k t)
-  (input: buffer8)
-  (sz: I32.t)
-  (h: HS.mem)
-  (res: Int32.t)
-  (h' : HS.mem)
-: GTot Type0
-= is_slice h input sz /\
-  M.modifies M.loc_none h h' /\ (
-    let pv = parse_from_slice p h input sz in
-    if I32.v res >= 0
-    then
-      Some? pv /\ (
-        let Some (_, consumed) = pv in
-        I32.v res == I32.v sz - consumed
-      )
-    else
-      None? pv
-  )
-
-[@unifier_hint_injective]
-inline_for_extraction
-let validator32
-  (#k: parser_kind)
-  (#t: Type0)
-  (p: parser k t)
-: Tot Type0
-= (input: buffer8) ->
-  (sz: I32.t) ->
-  HST.Stack I32.t
-  (requires (fun h ->
-    is_slice h input sz
-  ))
-  (ensures (fun h res h' ->
-    validator32_postcond p input sz h res h'
-  ))
-
-inline_for_extraction
-let validate32
-  (#k: parser_kind)
-  (#t: Type0)
-  (#p: parser k t)
-  (v: validator32 p)
-  (input: buffer8)
-  (sz: I32.t)
-: HST.Stack bool
-  (requires (fun h ->
-    is_slice h input sz
-  ))
-  (ensures (fun h res h' ->
-    is_slice h input sz /\
-    M.modifies M.loc_none h h' /\ (
-    let pv = parse_from_slice p h input sz in
-    res == Some? pv
- )))
-= let res = v input sz in
-  not (res `I32.lt` 0l)
-
-inline_for_extraction
-let ghost_parse_from_validator32
-  (#k: parser_kind)
-  (#t: Type0)
-  (#p: parser k t)
-  (v: validator32 p)
-  (input: buffer8)
-  (sz: I32.t)
-: HST.Stack (option (Ghost.erased t))
-  (requires (fun h ->
-    is_slice h input sz
-  ))
-  (ensures (fun h res h' ->
-    is_slice h input sz /\
-    M.modifies M.loc_none h h'  /\
-    res == (match parse_from_slice p h input sz with
-    | Some (x, _) -> Some (Ghost.hide x)
-    | _ ->  None
-  )))
-= let h = HST.get () in
-  if validate32 v input sz
-  then begin
-    let f () : GTot t =
-      let (Some (x, _)) = parse_from_slice p h input sz in
-      x
-    in
-    Some (Ghost.elift1 f (Ghost.hide ()))
-  end
-  else None
-
-inline_for_extraction
-let ghost_parse32
-  (#k: parser_kind)
-  (#t: Type0)
-  (p: parser k t)
-  (input: buffer8)
-: HST.Stack (Ghost.erased t)
-  (requires (fun h -> B.live h input /\ Some? (parse p (B.as_seq h input))))
-  (ensures (fun h res h' -> h == h' /\ (let (Some (x, _)) = parse p (B.as_seq h input) in res == Ghost.hide x)))
-= let h = HST.get () in
-  let f () : GTot t =
-    let (Some (x, _)) = parse p (B.as_seq h input) in
-    x
-  in
-  Ghost.elift1 f (Ghost.hide ())
-
-inline_for_extraction
-let parser32
-  (#k: parser_kind)
-  (#t: Type0)
-  (p: parser k t)
-: Tot Type0
-= (input: buffer8) ->
-  HST.Stack t
-  (requires (fun h ->
-    B.live h input /\
-    Some? (parse p (B.as_seq h input))
-  ))
-  (ensures (fun h res h' ->
-    M.modifies M.loc_none h h' /\
-    B.live h' input /\ (
-    let ps = parse p (B.as_seq h input) in
-    let (Some (res', _)) = ps in
-    res == res'
-  )))
-
-inline_for_extraction
-let validator_nochk32
-  (#k: parser_kind)
-  (#t: Type0)
-  (p: parser k t)
-: Tot Type0
-= (input: buffer8) ->
-  HST.Stack U32.t
-  (requires (fun h ->
-    B.live h input /\
-    Some? (parse p (B.as_seq h input))
-  ))
-  (ensures (fun h res h' ->
-    M.modifies M.loc_none h h' /\
-    B.live h' input /\
-    U32.v res <= B.length input /\ (
-    let (Some (x, res')) = parse p (B.as_seq h input) in
-    U32.v res == res'
-  )))
-
-inline_for_extraction
-let accessor
-  (#k1: parser_kind)
-  (#t1: Type)
-  (p1: parser k1 t1)
-  (#k2: parser_kind)
-  (#t2: Type)
-  (p2: parser k2 t2)
-  (rel: (t1 -> t2 -> GTot Type0))
-: Tot Type
-= (input: buffer8) ->
-  HST.Stack buffer8
-  (requires (fun h ->
-    B.live h input /\
-    Some? (parse p1 (B.as_seq h input))
-  ))
-  (ensures (fun h res h' ->
-    M.modifies (M.loc_none) h h' /\
-    B.live h' input /\
-    B.includes input res /\ (
-    let Some (x1, _) = parse p1 (B.as_seq h input) in
-    let ps2 = parse p2 (B.as_seq h res) in
-    Some? ps2 /\ (
-    let Some (x2, _) = ps2 in
-    rel x1 x2
-  ))))
-
-inline_for_extraction
-let read_from_buffer
-  (#k1: parser_kind)
-  (#t1: Type)
-  (#p1: parser k1 t1)
-  (#k2: parser_kind)
-  (#t2: Type)
-  (#p2: parser k2 t2)
-  (#rel: (t1 -> t2 -> GTot Type0))
-  (a12: accessor p1 p2 rel)
-  (p2' : parser32 p2)
-  (input: buffer8)
-: HST.Stack t2
-  (requires (fun h ->
-    B.live h input /\
-    Some? (parse p1 (B.as_seq h input))
-  ))
-  (ensures (fun h y h' ->
-    M.modifies M.loc_none h h' /\ (
-    let (Some (x, _)) = parse p1 (B.as_seq h input) in
-    rel x y
-  )))
-= p2' (a12 input)
-
-inline_for_extraction
-let serializer32
-  (#k: parser_kind)
-  (#t: Type)
-  (#p: parser k t)
-  (s: serializer p)
-: Tot Type
-= (b: buffer8) ->
-  (lo: U32.t) ->
-  (v: t) ->
-  HST.Stack unit
-  (requires (fun h -> B.live h b /\ U32.v lo + Seq.length (serialize s v) <= B.length b))
-  (ensures (fun h _ h' ->
-    let len = U32.uint_to_t (Seq.length (serialize s v)) in
-    M.modifies (loc_jbuffer b lo (U32.add lo len)) h h' /\
-    B.live h' b /\
-    exactly_contains_valid_data h' p b lo v (U32.add lo len)
-  ))
-
-inline_for_extraction
-let serializer32_fail
-  (#k: parser_kind)
-  (#t: Type)
-  (#p: parser k t)
-  (s: serializer p)
-: Tot Type
-= (b: buffer8) ->
-  (len: I32.t { I32.v len == B.length b } ) ->
-  (lo: I32.t) ->
-  (v: t) ->
-  HST.Stack I32.t
-  (requires (fun h -> B.live h b /\ I32.v lo <= I32.v len))
-  (ensures (fun h hi h' ->
-    B.live h' b /\
-    contains_valid_serialized_data_or_fail h' s b lo v hi /\
-    M.modifies (loc_ibuffer b lo hi) h h'
-  ))
-
-
-(* Stateful serializers for constant-size parsers *)
-
-inline_for_extraction
-let serializer32_fail_of_serializer
-  (#k: parser_kind)
-  (#t: Type)
-  (#p: parser k t)
-  (#s: serializer p)
-  (s32: serializer32 s)
-  (psz: I32.t { k.parser_kind_high == Some k.parser_kind_low /\ k.parser_kind_low == I32.v psz } ) 
-: Tot (serializer32_fail s)
-= fun out (len: I32.t { I32.v len == B.length out } ) lo v ->
-  let h = HST.get () in
-  if lo `I32.lt` 0l
-  then begin
-    let res = lo in
-    let h' = HST.get () in
-    assert (contains_valid_serialized_data_or_fail h' s out lo v res);
-    res
-  end
-  else begin
-    assert (I32.v lo >= 0);
-    assert (I32.v len >= 0);
-    assert (I32.v lo <= I32.v len);
-    assert (Seq.length (serialize s v) == I32.v psz);
-    if (len `I32.sub` lo) `I32.lt` psz
-    then begin
-      let res = I32.int_to_t (-1) in
-      let h' = HST.get () in
-      assert (contains_valid_serialized_data_or_fail h' s out lo v res);
-      assert (B.modifies (B.loc_buffer (B.gsub out (Cast.int32_to_uint32 lo) (B.len out `U32.sub` Cast.int32_to_uint32 lo))) h h');
-      res
-    end else begin
-      assert (Seq.length (serialize s v) == I32.v psz);
-      assert (I32.v lo + Seq.length (serialize s v) <= I32.v len);
-      assert (U32.v (Cast.int32_to_uint32 lo) == I32.v lo);
-      assert (U32.v (Cast.int32_to_uint32 lo) + Seq.length (serialize s v) <= I32.v len);
-      assert (U32.v (Cast.int32_to_uint32 lo) + Seq.length (serialize s v) <= B.length out);
-      s32 out (Cast.int32_to_uint32 lo) v;
-      let h = HST.get () in
-      exactly_contains_valid_data_contains_valid_serialized_data_or_fail h s out (Cast.int32_to_uint32 lo) v (Cast.int32_to_uint32 (lo `I32.add` psz));
-      lo `I32.add` psz
-    end
-  end
-  
-(* Low-level serialization *)
-
-assume
-val valid (h: HS.mem) (b: LL.buffer8) (off: U32.t) (#k: parser_kind) (#t: Type) (p: parser k t) : GTot Type0
-
-assume
-val contents (h: HS.mem) (b: LL.buffer8) (off: U32.t) (#k: parser_kind) (#t: Type) (
